\section{Calculer (2 points)}


\begin{questions}
	\question[1] $\dfrac{1}{4} + \dfrac{5}{2} - \dfrac{3}{4} + 2$
	\begin{solution}
		\begin{eqnarray*}
			\dfrac{1}{4} + \dfrac{5}{2} - \dfrac{3}{4} + 2 &=& \dfrac{1}{4} + \dfrac{5\times 2}{2 \times 2} - \dfrac{3}{4} + \dfrac{2 \times 4}{1 \times 4} \\
			\dfrac{1}{4} + \dfrac{5}{2} - \dfrac{3}{4} + 2 &=& \dfrac{1}{4} + \dfrac{10}{4} - \dfrac{3}{4} + \dfrac{8}{4} \\
			\dfrac{1}{4} + \dfrac{5}{2} - \dfrac{3}{4} + 2 &=& \dfrac{1 + 10 - 3 + 8}{4} \\
			\dfrac{1}{4} + \dfrac{5}{2} - \dfrac{3}{4} + 2 &=& \dfrac{16}{4} \\
			\dfrac{1}{4} + \dfrac{5}{2} - \dfrac{3}{4} + 2 &=& 4 \\
		\end{eqnarray*}
	\end{solution}
	
	\question[1] $4 - \dfrac{7}{3} - \dfrac{3}{4} + \dfrac{7}{12}$
	\begin{solution}
		\begin{eqnarray*}
			4 - \dfrac{7}{3} - \dfrac{3}{4} + \dfrac{7}{12} &=& \dfrac{4 \times 12}{1 \times 12} - \dfrac{7\times 4}{3 \times 4} - \dfrac{3 \times 3}{4 \times 3} + \dfrac{7}{12} \\
			4 - \dfrac{7}{3} - \dfrac{3}{4} + \dfrac{7}{12} &=& \dfrac{48}{12} - \dfrac{28}{12} - \dfrac{9}{12} + \dfrac{7}{12} \\
			4 - \dfrac{7}{3} - \dfrac{3}{4} + \dfrac{7}{12} &=& \dfrac{48 - 28 - 9 + 7}{12} \\
			4 - \dfrac{7}{3} - \dfrac{3}{4} + \dfrac{7}{12} &=& \dfrac{18}{12} \\
			4 - \dfrac{7}{3} - \dfrac{3}{4} + \dfrac{7}{12} &=& \dfrac{3}{2} \\
		\end{eqnarray*}
	\end{solution}
\end{questions}
